examples/wip/general/ChainTraceAgreement.v
@@ -1,0 +1,308 @@
+From ConCert.Execution Require Import Blockchain.
+From ConCert.Examples.Wip.General Require Import Blockchain_modify_2.
+
+From ConCert.Utils Require Import Automation.
+From ConCert.Utils Require Import Extras.
+From ConCert.Examples.Wip.General Require Import BuildUtils_modify_2.
+From ConCert.Examples.Wip.General Require Import ChainTraceProperty.
+From ConCert.Examples.Wip.General Require Import ContractCommon_modify_2.
+From ConCert.Execution Require Import Monad.
+From ConCert.Execution Require Import ResultMonad.
+From ConCert.Execution Require Import Serializable.
+From ConCert.Execution Require Import ChainedList.
+From Stdlib Require Import List. Import ListNotations.
+From Stdlib Require Import ZArith.
+From Stdlib Require Import Lia.
+From Stdlib Require Import FunctionalExtensionality.
+
+Module Orig := ConCert.Execution.Blockchain.
+Module Mod  := Blockchain_modify_2.
+
+
+
+
+
+
+
+Section ChainTraceAgreement.
+  Context {BaseO : Orig.ChainBase}.
+
+  Local Instance BaseM : Mod.ChainBase :=
+    {|
+      Mod.Address := Orig.Address;
+      Mod.address_eqb := Orig.address_eqb;
+      Mod.address_eqb_spec := Orig.address_eqb_spec;
+      Mod.address_eqdec := Orig.address_eqdec;
+      Mod.address_countable := Orig.address_countable;
+      Mod.address_serializable := Orig.address_serializable;
+      Mod.address_is_contract := Orig.address_is_contract;
+    |}.
+
+  Section EraseLayer.
+    
+    Context (erase_wc : Mod.WeakContract -> Orig.WeakContract).
+
+    
+    Definition erase_chain (c : Mod.Chain) : Orig.Chain :=
+      {|
+        Orig.chain_height := Mod.chain_height c;
+        Orig.current_slot := Mod.current_slot c;
+        Orig.finalized_height := Mod.finalized_height c;
+      |}.
+
+    
+    Definition erase_ctx (ctx : Mod.ContractCallContext) : Orig.ContractCallContext :=
+      {|
+        Orig.ctx_origin := Mod.ctx_origin ctx;
+        Orig.ctx_from := Mod.ctx_from ctx;
+        Orig.ctx_contract_address := Mod.ctx_contract_address ctx;
+        Orig.ctx_contract_balance := Mod.ctx_contract_balance ctx;
+        Orig.ctx_amount := Mod.ctx_amount ctx;
+      |}.
+
+    
+    Definition erase_ab (ab : Mod.ActionBody) : Orig.ActionBody :=
+      match ab with
+      | Mod.act_transfer to amount => Orig.act_transfer to amount
+      | Mod.act_call to amount msg => Orig.act_call to amount msg
+      | Mod.act_deploy amount wc setup => Orig.act_deploy amount (erase_wc wc) setup
+      end.
+
+    
+    Definition erase_act (a : Mod.Action) : Orig.Action :=
+      {|
+        Orig.act_origin := Mod.act_origin a;
+        Orig.act_from := Mod.act_from a;
+        Orig.act_body := erase_ab (Mod.act_body a);
+      |}.
+
+    
+    Definition erase_env (e : Mod.Environment) : Orig.Environment :=
+      {|
+        Orig.env_chain := erase_chain (Mod.env_chain e);
+        Orig.env_account_balances := Mod.env_account_balances e;
+        Orig.env_contracts := fun a => option_map erase_wc (Mod.env_contracts e a);
+        Orig.env_contract_states := Mod.env_contract_states e;
+      |}.
+
+    
+    Definition erase_state (st : Mod.ChainState) : Orig.ChainState :=
+      {|
+        Orig.chain_state_env := erase_env (Mod.chain_state_env st);
+        Orig.chain_state_queue := map erase_act (Mod.chain_state_queue st);
+      |}.
+
+(* Mod.BlockHeader -> Orig.BlockHeader *)
+Definition erase_header (h : Mod.BlockHeader) : Orig.BlockHeader :=
+  {|
+    Orig.block_height := Mod.block_height h;
+    Orig.block_slot := Mod.block_slot h;
+    Orig.block_finalized_height := Mod.block_finalized_height h;
+    Orig.block_reward := Mod.block_reward h;
+    Orig.block_creator := Mod.block_creator h;
+  |}.
+
+  Lemma IsValidNextBlock_sound (h : Mod.BlockHeader) (c : Mod.Chain) :
+    Mod.IsValidNextBlock h c ->
+    Orig.IsValidNextBlock (erase_header h) (erase_chain c).
+  Proof.
+    intros H; destruct H as [vh vs vfh vc vr].
+    refine
+      {|
+        Orig.valid_height := _;
+        Orig.valid_slot := _;
+        Orig.valid_finalized_height := _;
+        Orig.valid_creator := _;
+        Orig.valid_reward := _;
+      |};
+      cbn [erase_header erase_chain] in *; assumption.
+  Qed.
+
+    
+    Local Coercion erase_state : Mod.ChainState >-> Orig.ChainState.
+    Local Coercion erase_env   : Mod.Environment >-> Orig.Environment.
+    Local Coercion erase_act   : Mod.Action >-> Orig.Action.
+
+  Lemma act_is_from_account_sound (a : Mod.Action) :
+    Mod.act_is_from_account a ->
+    Orig.act_is_from_account (erase_act a).
+  Proof.
+    unfold Mod.act_is_from_account, Orig.act_is_from_account.
+    cbn [erase_act]; auto.
+  Qed.
+
+  Lemma act_origin_is_eq_from_sound (a : Mod.Action) :
+    Mod.act_origin_is_eq_from a ->
+    Orig.act_origin_is_eq_from (erase_act a).
+  Proof.
+    unfold Mod.act_origin_is_eq_from, Orig.act_origin_is_eq_from.
+    cbn [erase_act]; auto.
+  Qed.
+
+  Lemma Forall_act_is_from_account_sound (acts : list Mod.Action) :
+    Forall Mod.act_is_from_account acts ->
+    Forall Orig.act_is_from_account (map erase_act acts).
+  Proof.
+    induction 1; cbn; constructor; auto using act_is_from_account_sound.
+  Qed.
+
+  Lemma Forall_act_origin_is_eq_from_sound (acts : list Mod.Action) :
+    Forall Mod.act_origin_is_eq_from acts ->
+    Forall Orig.act_origin_is_eq_from (map erase_act acts).
+  Proof.
+    induction 1; cbn; constructor; auto using act_origin_is_eq_from_sound.
+  Qed.
+
+  Lemma EnvironmentEquiv_sound (e1 e2 : Mod.Environment) :
+    Mod.EnvironmentEquiv e1 e2 ->
+    Orig.EnvironmentEquiv (erase_env e1) (erase_env e2).
+  Proof.
+    intro Heq; destruct Heq as [Hc Hb Hcon Hst].
+    apply Orig.build_env_equiv; cbn.
+    - now rewrite Hc.
+    - intro a; exact (Hb a).
+    - intro a; now rewrite (Hcon a).
+    - intro a; exact (Hst a).
+  Qed.
+
+  
+
+
+  Lemma EnvironmentEquiv_erase_add_new_block (h : Mod.BlockHeader) (e : Mod.Environment) :
+    Orig.EnvironmentEquiv (erase_env (Mod.add_new_block_to_env h e))
+                          (Orig.add_new_block_to_env (erase_header h) (erase_env e)).
+  Proof.
+    apply Orig.build_env_equiv; cbn; try reflexivity.
+  Qed.
+
+    
+
+
+
+
+
+    Context
+      (ActionEvaluation_sound :
+         forall (prev : Mod.Environment) (act : Mod.Action)
+                (new : Mod.Environment) (new_acts : list Mod.Action),
+           Mod.ActionEvaluation prev act new new_acts ->
+           Orig.ActionEvaluation (erase_env prev) (erase_act act)
+                                 (erase_env new) (map erase_act new_acts)).
+
+    
+
+
+
+
+
+    Lemma ActionChainStep_to_OrigChainStep (st1 st2 : Mod.ChainState) :
+      Mod.ActionChainStep st1 st2 ->
+      Orig.ChainStep st1 st2.
+    Proof.
+      intro H.
+      inversion H as [act acts new_acts Hq Heval Hq']; subst.
+      eapply Orig.step_action
+        with (act := erase_act act)
+             (acts := map erase_act acts)
+             (new_acts := map erase_act new_acts).
+      - 
+        cbn. rewrite Hq. cbn. reflexivity.
+      - 
+        exact (ActionEvaluation_sound st1 act st2 new_acts Heval).
+      - 
+        cbn. rewrite Hq'. now rewrite map_app.
+    Qed.
+
+  Lemma ActionChainTrace_to_OrigChainTrace (st1 st2 : Mod.ChainState) :
+    Mod.ActionChainTrace st1 st2 ->
+    Orig.ChainTrace st1 st2.
+  Proof.
+    intro action_trace. remember st1; induction action_trace; subst.
+    constructor. 
+    specialize_hypotheses. 
+    apply ActionChainStep_to_OrigChainStep in l.
+    apply (snoc IHaction_trace l).
+  Qed.
+
+  
+
+
+
+  Lemma ModChainStep_to_OrigChainTrace (st1 st2 : Mod.ChainState) :
+    Mod.reachable st1 -> 
+    Mod.ChainStep st1 st2 ->
+    Orig.ChainTrace st1 st2. 
+  Proof.
+    intros reach step. 
+    destruct_chain_step. 
+    - enough (Orig.ChainStep st1 st2) as step_orig.
+      { apply (snoc clnil step_orig). }
+      apply (f_equal (map erase_act)) in queue_prev. cbn in queue_prev.
+      eapply (Orig.step_block) with (header := erase_header header); eauto.
+      + (* 2/5: IsValidNextBlock *)
+        change (Orig.IsValidNextBlock (erase_header header)
+                (erase_chain (Mod.env_chain (Mod.chain_state_env st1)))).
+        apply IsValidNextBlock_sound. exact valid_header.
+      + (* 3/5: Forall act_is_from_account *)
+        change (Forall Orig.act_is_from_account
+                (map erase_act (Mod.chain_state_queue st2))).
+        apply Forall_act_is_from_account_sound. exact acts_from_accs.
+      + (* 4/5: Forall act_origin_is_eq_from *)
+        change (Forall Orig.act_origin_is_eq_from
+                (map erase_act (Mod.chain_state_queue st2))).
+        apply Forall_act_origin_is_eq_from_sound. exact origin_correct.
+      + (* 5/5: EnvironmentEquiv *)
+        
+        eapply RelationClasses.transitivity.
+        * exact (EnvironmentEquiv_sound _ _ env_eq).
+        * apply EnvironmentEquiv_erase_add_new_block.
+    - apply ActionChainTrace_to_OrigChainTrace; auto. 
+    - specialize (queue_from_account st1 reach) as from_accs. 
+      rewrite_queue.
+      apply Forall_cons_iff in from_accs as (from_acc & _).
+      enough (Orig.ChainStep st1 st2) as step_orig. 
+      { apply (snoc clnil step_orig). }
+      apply (f_equal (map erase_act)) in queue_prev. 
+      apply (f_equal (map erase_act)) in queue_new. cbn in *.
+      eapply Orig.step_action_invalid; eauto.
+      + exact (EnvironmentEquiv_sound _ _ env_eq).
+      + 
+        enough (
+         (forall bstate new_acts, 
+          Orig.ActionEvaluation st1 act bstate new_acts -> 
+                                              False) ->
+         (forall bstate,
+          bstate.(Mod.chain_state_queue) = acts ->
+          Mod.ActionChainTrace st1 bstate -> 
+                                               False) 
+        ). 
+        intros * no_eval.
+        eapply H.
+        (* eapply (no_action_trace).  *)
+         
+      all : admit. 
+  Admitted.
+
+  Lemma ModChainTrace_to_OrigChainTrace (st1 st2 : Mod.ChainState) :
+    Mod.reachable st1 -> 
+    Mod.ChainTrace st1 st2 ->
+    Orig.ChainTrace st1 st2. 
+  Proof.
+    intros reach trace. remember st1; induction trace; subst. 
+    constructor. 
+    specialize_hypotheses. apply ModChainStep_to_OrigChainTrace in l. 
+    apply (clist_app IHtrace l). 
+    eapply (reachable_trans); eauto. 
+  Qed.  
+
+    
+
+
+
+
+
+
+
+
+  End EraseLayer.
+End ChainTraceAgreement.
